theory/Util/IntMap.v
@@ -187,7 +187,6 @@ Proof.
         now inversion ndps.
 Qed.
 
-(*TODO*)
 Global Instance int_Discrete : Discrete int.
 Proof.
   constructor.
@@ -326,9 +325,6 @@ Proof.
   - simpl in *.
     destruct HIn.
     + inversion H1; subst.
-
-
-
       destruct (in_dec x' (map fst qs)).
       * apply (IHqs (hash_add x' y' m));
           [exact (functional_tail ndkeys)|].
@@ -357,3 +353,318 @@ Global Instance AssocList_SM : IntMap (AL.t int) := {|
   size_empty X := AL.size_empty;
   size_add X := AL.size_add;
   |}.
+
+Section CondHashFacts.
+
+Context {X : Type}.
+Context {Y : Type}.
+Context {P : X -> Prop}.
+Context {M : Type -> Type}.
+
+Context `{IntMap M}.
+Context `{CondIntHash X P}.
+
+Definition chash_add : X -> Y -> M Y -> M Y :=
+  fun x => add (chash x).
+
+Definition chash_lookup : X -> M Y -> option Y :=
+  fun x => lookup (chash x).
+
+Lemma chash_lookup_empty : forall x, chash_lookup x (empty : M Y) = None.
+Proof.
+  intro.
+  apply lookup_empty.
+Qed.
+
+Lemma chash_lookup_add : forall (x : X) (y : Y) m, chash_lookup x (chash_add x y m) = Some y.
+Proof.
+  intros.
+  apply lookup_add.
+Qed.
+
+Lemma chash_lookup_add_neq : forall (x x' : X) (y : Y) m,
+  x <> x' -> P x -> P x' ->
+  chash_lookup x (chash_add x' y m) = chash_lookup x m.
+Proof.
+  intros x x' y m Hxx' px px'.
+  apply lookup_add_neq.
+  intro Hhash.
+  apply Hxx'.
+  now apply chash_inj.
+Qed.
+
+Lemma chash_size_add :
+  forall (x : X) (y : Y) m,
+    size (chash_add x y m) =
+      match chash_lookup x m with
+      | Some _ => size m
+      | None => S (size m)
+      end.
+Proof.
+  intros.
+  apply size_add.
+Qed.
+
+Fixpoint chash_adds (ps : list (X * Y)) (m : M Y) {struct ps} : M Y :=
+  match ps with
+  | [] => m
+  | (x,y) :: qs => chash_adds qs (chash_add x y m)
+  end.
+
+Inductive cgood : M Y -> Prop :=
+  | cgood_e : cgood empty
+  | cgood_a {x y m} : cgood m -> chash_lookup x m = None -> P x -> cgood (chash_add x y m).
+
+Fixpoint cgood_as {ps : list (X * Y)}
+  {m : M Y} (pf : cgood m) (nd : NoDup (map fst ps))
+  (pps : Forall P (map fst ps))
+  (disj : forall x y, In (x,y) ps -> chash_lookup x m = None) {struct ps}
+  : cgood (chash_adds ps m).
+Proof.
+  induction ps as [|[x y] qs].
+  - exact pf.
+  - inversion pps.
+    simpl.
+    apply cgood_as; auto.
+    + apply cgood_a; auto.
+      apply (disj x y); now left.
+    + now inversion nd.
+    + intros x' y' HIn.
+      rewrite chash_lookup_add_neq; auto.
+      * apply (disj x' y'); now right.
+      * simpl in nd; inversion nd.
+        intro Heq.
+        apply H7.
+        rewrite <- Heq.
+        rewrite in_map_iff.
+        exists (x', y'); split; auto.
+      * rewrite Forall_forall in H4.
+        apply H4.
+        apply in_map with (f := fst) in HIn.
+        auto.
+Qed.
+
+Record cmap_list_equiv (m : M Y) (ps : list (X * Y)) : Prop := {
+  cto_list_size : size m = List.length ps;
+  ckeys_unique : NoDup (map fst ps);
+  clookup_in {x y} : P x -> chash_lookup x m = Some y <-> In (x,y) ps;
+  }.
+
+Lemma chash_adds_add {ps : list (X * Y)} : forall x y m,
+  chash_add x y (chash_adds ps m) = chash_adds (ps ++ [(x,y)]) m.
+Proof.
+  induction ps; intros.
+  - reflexivity. 
+  - simpl.
+    destruct a.
+    now rewrite IHps.
+Qed.
+
+Lemma chash_size_add_le (x : X) (y : Y) : forall m : M Y,
+  size m <= size (chash_add x y m).
+Proof.
+  intro.
+  rewrite chash_size_add.
+  destruct chash_lookup; lia.
+Qed.
+
+Lemma chash_size_adds_le (ps : list (X * Y)) : forall m : M Y,
+  size m <= size (chash_adds ps m).
+Proof.
+  induction ps as [|[x y] qs].
+  - intro; simpl. lia.
+  - intros; simpl.
+    simpl.
+    apply (PeanoNat.Nat.le_trans _ (size (chash_add x y m))).
+    + apply chash_size_add_le.
+    + apply IHqs.
+Qed.
+
+Lemma chash_adds_ne_pos (ps : list (X * Y)) : forall (x : X) (y : Y),
+  In (x,y) ps -> size (chash_adds ps empty) > 0.
+Proof.
+  destruct ps as [|[x' y'] qs]; intros.
+  - destruct H1.
+  - simpl.
+    pose proof (chash_size_adds_le qs (chash_add x' y' empty)).
+    rewrite chash_size_add in H2.
+    rewrite chash_lookup_empty in H2.
+    lia.
+Qed.
+
+Lemma chash_size_adds (ps : list (X * Y)) : forall m : M Y,
+  NoDup (map fst ps) ->
+  Forall P (map fst ps) ->
+  (forall x, In x (map fst ps) -> chash_lookup x m = None) ->
+  size (chash_adds ps m) = List.length ps + size m.
+Proof.
+  induction ps as [|[x y] qs]; intros m ndps pps Hpsm.
+  - reflexivity.
+  - simpl.
+    inversion pps.
+    rewrite IHqs; auto.
+    + rewrite chash_size_add.
+      rewrite Hpsm.
+      * apply PeanoNat.Nat.add_succ_r.
+      * left; reflexivity.
+    + now inversion ndps.
+    + intros.
+      rewrite chash_lookup_add_neq; auto.
+      * apply Hpsm.
+        right; auto.
+      * intro Hx0x.
+        rewrite Hx0x in H5.
+        now inversion ndps.
+      * rewrite Forall_forall in H4.
+        apply H4.
+        auto.
+Qed.
+
+Lemma chash_lookup_adds_invert (ps : list (X * Y)) : forall (m : M Y)
+  (x : X) (y : Y), P x ->
+  Forall P (map fst ps) ->
+  chash_lookup x (chash_adds ps m) = Some y ->
+  {In (x,y) ps} + {chash_lookup x m = Some y}.
+Proof.
+  induction ps as [|[x y] qs]; intros m x' y' px pps Hx'.
+  - right. exact Hx'.
+  - simpl in Hx'.
+    simpl in pps.
+    rewrite Forall_cons_iff in pps.
+    destruct pps.
+    destruct (IHqs _ _ _ px H2 Hx').
+    + left; now right.
+    + destruct (eq_dec (chash x') (chash x)).
+      * assert (x' = x) as Hx'x.
+        { apply chash_inj; auto. }
+        rewrite Hx'x in e.
+        rewrite chash_lookup_add in e.
+        left; left; congruence.
+      * rewrite chash_lookup_add_neq in e; auto.
+        intro Hx'x.
+        now rewrite Hx'x in n.
+Defined.
+
+Lemma cgood_to_list (m : M Y) (g : cgood m) : exists (ps : list (X * Y)),
+  cmap_list_equiv m ps.
+Proof.
+  induction g.
+  - exists nil; constructor.
+    + now rewrite size_empty.
+    + constructor.
+    + intros x y.
+      unfold chash_lookup.
+      now rewrite lookup_empty.
+  - destruct IHg as [ps [tl_sz key_un l_in]].
+    exists ((x,y) :: ps); constructor.
+    + unfold chash_add.
+      unfold chash_lookup in H1.
+      rewrite size_add.
+      rewrite H1.
+      simpl; congruence.
+    + simpl; constructor; auto.
+      intro HIn.
+      rewrite in_map_iff in HIn.
+      destruct HIn as [[str x'] [Hx1 Hx2]].
+      simpl in *.
+      rewrite Hx1 in Hx2.
+      rewrite <- l_in in Hx2; congruence.
+    + intros.
+      unfold chash_lookup, chash_add.
+      destruct (eq_dec (chash x0) (chash x)).
+      * rewrite e.
+        rewrite lookup_add.
+        split; intro.
+        -- apply chash_inj in e; auto.
+           left; congruence.
+        -- destruct H4; [congruence|].
+           rewrite <- l_in in H4; auto.
+           apply chash_inj in e; auto.
+           congruence.
+      * rewrite lookup_add_neq; auto.
+        unfold chash_lookup in l_in.
+        rewrite l_in; auto.
+        split; intro; [now right|].
+        destruct H4; auto.
+        congruence.
+Qed.
+
+Lemma chash_lookup_adds_None_invert {ps} (pps : Forall P (map fst ps)) : forall {m : M Y} {x : X}, P x ->
+  chash_lookup x (chash_adds ps m) = None ->
+  (~ In x (List.map fst ps)) /\
+  chash_lookup x m = None.
+Proof.
+  induction ps as [|[x y] qs]; intros m x' px' Hx'.
+  - split.
+    + intros [].
+    + exact Hx'.
+  - simpl in *.
+    rewrite Forall_cons_iff in pps.
+    destruct pps as [pps1 pps2].
+    destruct (IHqs pps2 _ _ px' Hx').
+    split.
+    + intros [|].
+      * rewrite H3 in H2.
+        now rewrite chash_lookup_add in H2.
+      * contradiction.
+    + destruct (eq_dec (chash x') (chash x)).
+      * apply chash_inj in e; auto.
+        rewrite e in H2.
+        now rewrite chash_lookup_add in H2.
+      * rewrite chash_lookup_add_neq in H2; auto.
+        congruence.
+Qed.
+
+Lemma chash_lookup_adds_nIn :
+  forall (ps : list (X * Y)) (x : X) m,
+    Forall P (map fst ps) -> P x ->
+    ~ In x (List.map fst ps) ->
+    chash_lookup x (chash_adds ps m) = chash_lookup x m.
+Proof.
+  intro ps.
+  induction ps as [|[x y] qs]; intros x' m pps px nIn.
+  - reflexivity.
+  - simpl.
+    rewrite IHqs; auto.
+    + rewrite chash_lookup_add_neq; auto.
+      * intro Hxx'; apply nIn.
+        left; symmetry; exact Hxx'.
+      * inversion pps; auto.
+    + inversion pps; auto.
+    + intro HIn; apply nIn.
+      right; auto.
+Qed.
+
+Lemma chash_lookup_adds `{Discrete X} (ps : list (X * Y)) : forall m : M Y,
+  functional ps ->
+  Forall P (map fst ps) ->
+  forall (x : X) (y : Y), In (x,y) ps ->
+  chash_lookup x (chash_adds ps m) = Some y.
+Proof.
+  induction ps as [|[x y] qs]; intros m ndkeys pps x' y' HIn.
+  - destruct HIn.
+  - simpl in *.
+    destruct HIn.
+    + inversion H1; subst.
+      rewrite Forall_cons_iff in pps.
+      destruct pps as [pps1 pps2].
+      destruct (in_dec x' (map fst qs)).
+      * apply (IHqs (chash_add x y m)); auto;
+          [exact (functional_tail ndkeys)|].
+        unfold functional in ndkeys.
+        rewrite in_map_iff in i.
+        destruct i as [[u v] [Heq HIn]].
+        simpl in Heq; subst.
+        rewrite (ndkeys x' y' v); auto.
+        -- now left.
+        -- now right.
+      * rewrite chash_lookup_adds_nIn; auto.
+        -- inversion H2.
+           apply chash_lookup_add.
+        -- congruence.
+    + rewrite Forall_cons_iff in pps; destruct pps.
+      apply IHqs; auto.
+      exact (functional_tail ndkeys).
+Qed.
+
+End CondHashFacts.
